pulse/lib/steel/pulse/Pulse.Checker.Auto.Framing.fst
@@ -1,0 +1,35 @@
+module Pulse.Checker.Auto.Framing
+open Pulse.Checker.Auto.Util
+open Pulse.Syntax
+open Pulse.Typing
+open Pulse.Checker.VPropEquiv
+open Pulse.Typing.Metatheory
+module F = Pulse.Checker.Framing
+
+
+let step_match : prover_step_t = 
+  fun #g #o (p:prover_state g o) ->
+    let res = F.all_matches g p.unmatched_pre p.remaining_ctxt in
+    match res.matched with
+    | [] -> None
+    | _ ->
+      let matched_pre = Tm_Star (list_as_vprop res.matched) p.matched_pre in
+        // remaining_ctxt ~ res.ctxt' * res.matched
+      let veq 
+        : vprop_equiv_x g tm_unit 
+                          (Tm_Star (list_as_vprop p.remaining_ctxt) p.matched_pre)
+                          (Tm_Star (list_as_vprop res.unmatched_q) matched_pre)
+        = magic ()
+      in
+        // p.unmatched_pre ~ res.unmatched @ res.matched
+      let pre_equiv
+          : vprop_equiv g (comp_pre p.c) (Tm_Star (list_as_vprop res.unmatched_p) matched_pre)
+          = magic ()
+      in
+      let proof_steps_typing = st_typing_equiv_post p.proof_steps_typing veq in
+      Some 
+        { p with unmatched_pre = res.unmatched_p;
+                 matched_pre;
+                 remaining_ctxt = res.unmatched_q;
+                 proof_steps_typing;
+                 pre_equiv }
